Examples/Ratchet/Instance.lean
@@ -1,0 +1,84 @@
+module
+
+public import Examples.Ratchet.Specification
+public import Examples.Ratchet.Proof
+
+namespace DY.Example.Ratchet
+
+public section
+
+#combine +toplevel into BytesFunctor, BytesLength, attackerKnowledge from
+  Random,
+  Literal,
+  Concat,
+  Hash,
+  Signature,
+  DiffieHellman,
+  KdfExtract,
+  KdfExpand,
+
+instance: HasExecBytes where
+
+#combine +toplevel into
+  ExecEntryT,
+  baseAttackerKnowledge,
+from
+  Network,
+  Random,
+  ProtocolEvent RatchetEvent,
+  PersistentLocalState.CompromisableState StateMyTurn,
+  PersistentLocalState.CompromisableState StateOtherTurn,
+  LongTermKeys "Ratchet PKI",
+
+instance: HasExecTrace where
+
+#combine +toplevel into
+  ProofEntryT,
+from
+  Network,
+  Random,
+  ProtocolEvent RatchetEvent,
+  PersistentLocalState.CompromisableState StateMyTurn,
+  PersistentLocalState.CompromisableState StateOtherTurn,
+  LongTermKeys "Ratchet PKI",
+
+instance: HasProofTrace where
+
+#combine +toplevel into BytesInvariants, BytesInvariantsProofs from
+  Random,
+  Literal,
+  Concat,
+  Hash,
+  Signature,
+  DiffieHellman,
+  KdfExtract,
+  KdfExpand,
+
+instance: HasBytesInvariants where
+
+#combine +toplevel into
+  SubTraceInvariant,
+  SubBaseAttackerKnowledgeTheorem,
+from
+  Network,
+  Random,
+  ProtocolEvent RatchetEvent,
+  PersistentLocalState.CompromisableState StateMyTurn,
+  PersistentLocalState.CompromisableState StateOtherTurn,
+  LongTermKeys "Ratchet PKI",
+
+#combine +toplevel into SubAttackerKnowledgeTheorem from
+  Random,
+  Literal,
+  Concat,
+  Hash,
+  Signature,
+  DiffieHellman,
+  KdfExtract,
+  KdfExpand,
+
+instance: HasTraceInvariant where
+
+end
+
+end DY.Example.Ratchet
